theories/L6_PCPS/identifiers.v
@@ -1,5 +1,5 @@
-Require Import cps cps_util set_util.
-Require Import List BinNat Relations Coq.MSets.MSetRBT List.
+Require Import List BinNat Relations Coq.MSets.MSetRBT List Ensembles.
+Require Import cps cps_util set_util Ensembles_util.
 Import ListNotations.
 
 Import PS.
@@ -7,151 +7,273 @@ Import PS.
 Definition FVSet := PS.t.
 
 
-(** [f] is a function defined in [B] *)
-Fixpoint name_in_fundefs f (B : fundefs) :=
+Instance DecidableSingleton_var x : Decidable (Singleton var x).
+Proof.
+  constructor. intros x'.
+  destruct (var_dec x x'); subst. left; constructor.
+  right. intros Hc. inv Hc; eauto.
+Qed.
+
+(** [name_in_fundefs B] is the set of the names of the functions in [B] *)
+Fixpoint name_in_fundefs (B : fundefs) : Ensemble var :=
   match B with
-    | Fnil => False
+    | Fnil => Empty_set var
     | Fcons f' _ _ _ B =>
-      f' = f \/ name_in_fundefs f B
+      Union var (Singleton var f') (name_in_fundefs B)
   end.
 
-Lemma name_in_fundefs_dec x B :
-  {name_in_fundefs x B} + {~ name_in_fundefs x B}.
+Instance Decidable_name_in_fundefs (B : fundefs) : Decidable (name_in_fundefs B).
 Proof.
-  induction B.
+  constructor.
+  induction B; intros x.
   - destruct (Coqlib.peq x v); subst.
-    left. left; eauto.
-    inv IHB. left. right; eauto.
-    right. intros Hc. apply H. inv Hc; congruence.
+    left. left. eauto.
+    destruct (IHB x). left. right; eauto.
+    right. intros Hc. inv Hc. inv H0; congruence. 
+    exfalso. eauto.
   - right. intros Hc; inv Hc.
 Qed.
 
-
-(** The function [(f, tau, xs, e)] is defined in [B] *)
-Fixpoint fun_in_fundefs f tau xs e (B : fundefs) :=
+(** [fun+in_fundefs B] is the set of functions defined in [B] *)
+Fixpoint fun_in_fundefs  (B : fundefs) : Ensemble (var * type * list var * exp) :=
   match B with
-    | Fnil => False
-    | Fcons f' tau' xs' e' B =>
-      (f' = f /\ tau' = tau /\ xs' = xs /\ e = e') \/
-      fun_in_fundefs f tau xs e B
+    | Fnil => Empty_set _
+    | Fcons f tau xs e B =>
+      Union _ (Singleton _ (f, tau, xs, e))
+            (fun_in_fundefs B)
   end.
 
 (** [find_def] is correct w.r.t. [fun_in_fundefs] *)
 Lemma find_def_correct f B tau xs e :
   find_def f B = Some (tau, xs, e) ->
-  fun_in_fundefs f tau xs e B.
+  fun_in_fundefs B (f, tau, xs, e).
 Proof.
   induction B; simpl; intros H; try discriminate.
   destruct (M.elt_eq f v).
-  - inv H; eauto.
+  - inv H. left; eauto.
   - right; eauto.
 Qed.
     
-(** [occurs_free x e] iff [x] appears free in [e] *)
-Inductive occurs_free : var -> exp -> Prop :=
+(** [occurs_free e] is the set of free variables of [e] *)
+Inductive occurs_free : exp -> Ensemble var :=
 | Free_Econstr1 :
     forall y x tau t ys e,
       List.In y ys ->
-      occurs_free y (Econstr x tau t ys e)
+      occurs_free (Econstr x tau t ys e) y
 | Free_Econstr2 :
     forall y x tau t ys e,
       ~ x = y ->
-      occurs_free y e ->
-      occurs_free y (Econstr x tau t ys e)
+      occurs_free e y ->
+      occurs_free (Econstr x tau t ys e) y
 | Free_Ecase1 :
     forall x ys, 
-      occurs_free x (Ecase x ys)
+      occurs_free (Ecase x ys) x
 | Free_Ecase2 :  
     forall y x c e ys,
-      occurs_free y e ->
-      occurs_free y (Ecase x ((c, e) :: ys))
+      occurs_free e y ->
+      occurs_free (Ecase x ((c, e) :: ys)) y
 | Free_Ecase3 :  
     forall y x c e ys,
-      occurs_free y (Ecase x ys) ->
-      occurs_free y (Ecase x ((c, e) :: ys))
+      occurs_free (Ecase x ys) y ->
+      occurs_free (Ecase x ((c, e) :: ys)) y
 | Free_Eproj1 :
     forall y x tau n e,
-      occurs_free y (Eproj x tau n y e)
+      occurs_free (Eproj x tau n y e) y
 | Free_Eproj2 :
     forall y x tau n y' e,
       x <> y ->
-      occurs_free y e ->
-      occurs_free y (Eproj x tau n y' e)
+      occurs_free e y ->
+      occurs_free (Eproj x tau n y' e) y
 | Free_Efun1 :
     forall y defs e,
-      ~ (name_in_fundefs y defs) -> 
-      occurs_free y e ->
-      occurs_free y (Efun defs e)
+      ~ (name_in_fundefs defs y) -> 
+      occurs_free e y ->
+      occurs_free (Efun defs e) y
 | Free_Efun2 :
     forall y defs e, 
-      occurs_free_fundefs y defs ->
-      occurs_free y (Efun defs e)
+      occurs_free_fundefs defs y ->
+      occurs_free (Efun defs e) y
 | Free_Eapp1 :
     forall x ys,
-      occurs_free x (Eapp x ys)
+      occurs_free (Eapp x ys) x
 | Free_Eapp2 :
     forall y x ys,
       List.In y ys ->
-      occurs_free y (Eapp x ys)
+      occurs_free (Eapp x ys) y
 | Free_Eprim1 :
     forall y x tau p ys e,
       List.In y ys ->
-      occurs_free y (Eprim x tau p ys e)
+      occurs_free (Eprim x tau p ys e) y
 | Free_Eprim2 :
     forall y x tau p ys e,
       x <> y ->
-      occurs_free y e ->
-      occurs_free y (Eprim x tau p ys e)
-with occurs_free_fundefs : var -> fundefs -> Prop :=
+      occurs_free e y ->
+      occurs_free (Eprim x tau p ys e) y
+with occurs_free_fundefs : fundefs -> Ensemble var :=
 | Free_Fcons1 :
     forall x f tau ys e defs,  
       x <> f ->
       ~ (List.In x ys) ->
-      ~ (name_in_fundefs x defs) ->
-      occurs_free x e ->
-      occurs_free_fundefs x (Fcons f tau ys e defs)
+      ~ (name_in_fundefs defs x) ->
+      occurs_free e x ->
+      occurs_free_fundefs (Fcons f tau ys e defs) x
 | Free_Fcons2 :
     forall x f tau ys e defs,
-      occurs_free_fundefs x defs ->
+      occurs_free_fundefs defs x ->
       x <> f ->
-      occurs_free_fundefs x (Fcons f tau ys e defs).
+      occurs_free_fundefs (Fcons f tau ys e defs) x.
+
+Hint Constructors occurs_free.
+Hint Constructors occurs_free_fundefs.
 
 (** sanity check : The names of the functions cannot appear 
     free in a fundefs block *)
 Lemma fun_names_not_free_in_fundefs f defs :
-  name_in_fundefs f defs ->
-  ~ occurs_free_fundefs f defs.
+  name_in_fundefs defs f ->
+  ~ occurs_free_fundefs defs f.
 Proof.
-  intros Hname Hfree.
+  intros Hname Hfree. 
   induction Hfree; inversion Hname; eauto.
+  inv H3. eauto. inv H0; eauto.
 Qed.
 
-Lemma occurs_free_in_fun f tau xs e B x :
-  fun_in_fundefs f tau xs e B ->
-  occurs_free x e ->
-  List.In x xs \/ name_in_fundefs x B \/ occurs_free_fundefs x B.
+Lemma occurs_free_Econstr_Included x tau t ys e :
+  Included var (occurs_free e)
+           (Union var (occurs_free (Econstr x tau t ys e)) (Singleton var x)).
 Proof.
-  induction B; intros H Hfree; inv H.
-  - destruct H0 as [H1 [H2 [H3 H4]]]; subst.
-    destruct (Coqlib.peq x f); subst.
-    + right. left. constructor; eauto.
-    + destruct (in_dec var_dec x xs); eauto; subst.
-      destruct (name_in_fundefs_dec x B).
-      * right. left. right; eauto.
-      * right. right. constructor; eauto.
-  - destruct (Coqlib.peq x v); subst.
+  intros x' Hin.
+  destruct (var_dec x x'); subst; eauto.
+Qed.
+
+Lemma occurs_free_Eproj_Included x tau t y e :
+  Included var (occurs_free e)
+           (Union var (occurs_free (Eproj x tau t y e)) (Singleton var x)).
+Proof.
+  intros x' Hin.
+  destruct (var_dec x x'); subst; eauto.
+Qed.
+
+Lemma occurs_free_Eprim_Included x tau f ys e :
+  Included var (occurs_free e)
+           (Union var (occurs_free (Eprim x tau f ys e)) (Singleton var x)).
+Proof.
+  intros x' Hin.
+  destruct (var_dec x x'); subst; eauto.
+Qed.
+
+Lemma occurs_free_Efun_Included B e:
+  Included var (occurs_free e)
+           (Union var (occurs_free (Efun B e)) (name_in_fundefs B)).
+Proof.
+  intros x' Hin.
+  destruct (@Dec _ _ (Decidable_name_in_fundefs B) x'); subst; eauto.
+Qed.
+
+Lemma occurs_free_Ecase_Included P c x e :
+  List.In (c, e) P ->
+  Included var (occurs_free e)
+           (occurs_free (Ecase x P)).
+Proof.
+  intros Hin x' Hin'. induction P as [ | [c' e'] P IHP]; try now inv Hin.
+  inv Hin.
+  - inv H. constructor; eauto.
+  - eapply Free_Ecase3. eapply IHP; eauto.
+Qed.
+
+Lemma occurs_free_dec :
+  (forall e, Decidable (occurs_free e)) /\
+  (forall B, Decidable (occurs_free_fundefs B)).
+Proof.
+  exp_defs_induction IHe IHl IHdefs; try inv IHe; try inv IHl;
+  try inv IHdefs; constructor; intros x.
+  - destruct (in_dec var_dec x l); eauto.
+    destruct (var_dec x v); subst. right. intros Hc. inv Hc; eauto.
+    destruct (Dec x); eauto.
+    right. intros Hc. inv Hc; eauto.
+  - destruct (var_dec x v); subst; eauto.
+    right; intros Hc. inv Hc; congruence.
+  - destruct (var_dec x v); subst; eauto.
+    destruct (Dec x); eauto.
+    destruct (Dec0 x); eauto.
+    right. intros Hc. inv Hc; eauto.
+  - destruct (var_dec x v0); subst; eauto.
+    destruct (var_dec x v); subst. right. intros Hc. inv Hc; eauto.
+    destruct (Dec x); eauto.
+    right. intros Hc. inv Hc; eauto.
+  - destruct (Decidable_name_in_fundefs f2). destruct (Dec1 x).
+    right. intros Hc. inv Hc; eauto. eapply fun_names_not_free_in_fundefs; eauto.
+    destruct (Dec x); eauto.
+    destruct (Dec0 x); eauto.
+    right. intros Hc. inv Hc; eauto.
+  - destruct (in_dec var_dec x l); eauto.
+    destruct (var_dec x v); subst; eauto.
+    right. intros Hc. inv Hc; eauto.
+  - destruct (in_dec var_dec x l); eauto.
+    destruct (var_dec x v); subst. right. intros Hc. inv Hc; eauto.
+    destruct (Dec x); eauto.
+    right. intros Hc. inv Hc; eauto.
+  - destruct (Decidable_name_in_fundefs f5). destruct (Dec1 x).
+    right. intros Hc. inv Hc; eauto. eapply fun_names_not_free_in_fundefs; eauto.
+    destruct (var_dec x v); subst. right. intros Hc. inv Hc; eauto.
+    destruct (Dec0 x); eauto.
+    destruct (in_dec var_dec x l). right. intros Hc. inv Hc; eauto.
+    destruct (Dec x); eauto. right. intros Hc. inv Hc; eauto.
+  - right. intros Hc. inv Hc.
+Qed.
+    
+Instance Decidable_occurs_free e : Decidable (occurs_free e).
+Proof.
+  now apply occurs_free_dec.
+Qed.
+
+Instance Decidable_occurs_free_fundefs e : Decidable (occurs_free_fundefs e).
+Proof.
+  now apply occurs_free_dec.
+Qed.
+
+Lemma occurs_free_in_fun f tau xs e B :
+  fun_in_fundefs B (f, tau, xs, e) ->
+  Included var (occurs_free e) 
+           (Union var (FromList xs) (Union var (name_in_fundefs B)
+                                           (occurs_free_fundefs B))).
+Proof.
+  induction B; intros H; inv H.
+  - inv H0. intros x H.
+    destruct (Coqlib.peq x f); simpl; subst; eauto.
+    destruct (in_dec var_dec x xs); eauto; subst.
+    destruct (@Dec _ _ (Decidable_name_in_fundefs B) x); eauto.
+  - intros x H. destruct (Coqlib.peq x v); subst.
     + right; left. left; eauto.
-    + edestruct IHB as [H | [H | H]]; eauto.
-      * right. left. right; eauto.
-      * right. right. constructor 2; eauto.
+    + edestruct (IHB H0 x) as [H'| H']; eauto.
+      inv H1; eauto. right. left. right; eauto.
+Qed.
+
+Lemma find_def_name_in_fundefs f B v:
+  find_def f B = Some v ->
+  name_in_fundefs B f.
+Proof.
+  induction B; simpl; intros H; try now inv H.
+  destruct (M.elt_eq f v0); inv H.
+  left; eauto. right; eauto.
+Qed.
+
+
+Lemma name_in_fundefs_find_def_None f B:
+  ~ name_in_fundefs B f ->
+  find_def f B = None.
+Proof.
+  induction B; simpl; intros H; eauto.
+  destruct (M.elt_eq f v); subst.
+  - exfalso. apply H. now left.
+  - eapply IHB. intros Hc. apply H. now right.
 Qed.
       
-   
+
 Definition closed_exp (e : exp) : Prop :=
-  forall x, ~ (occurs_free x e).
+  Same_set var (occurs_free e) (Empty_set var).
 
 Definition closed_fundefs (defs : fundefs) : Prop :=
-  forall x, ~ (occurs_free_fundefs x defs).
+  Same_set var (occurs_free_fundefs defs) (Empty_set var).
 
 (** [funs_in_exp B e] iff [B] is a block of functions in [e] *)
 Inductive funs_in_exp : fundefs -> exp -> Prop :=
@@ -191,86 +313,247 @@ with funs_in_fundef : fundefs -> fundefs -> Prop :=
 (** all functions defined in an expression are closed *)
 Definition closed_fundefs_in_exp (e : exp) :=
   forall defs, funs_in_exp defs e -> closed_fundefs defs.
-
+  
 (** bound variables - alternative definition without lists or 
     number of occurences *)
-Inductive bound_var : var -> exp -> Prop :=
+Inductive bound_var : exp -> Ensemble var :=
 | Bound_Econstr1 :
     forall x tau t ys e,
-      bound_var x (Econstr x tau t ys e)
+      bound_var (Econstr x tau t ys e) x
 | Bound_Econstr2 :
     forall y x tau t ys e,
-      bound_var y e ->
-      bound_var y (Econstr x tau t ys e)
+      bound_var e y ->
+      bound_var (Econstr x tau t ys e) y
 | Bound_Eproj1 :
     forall x y tau n e,
-      bound_var x (Eproj x tau n y e)
+      bound_var (Eproj x tau n y e) x
 | Bound_Eproj2 :
     forall y x tau n y' e,
-      bound_var y e ->
-      bound_var y (Eproj x tau n y' e)
+      bound_var e y ->
+      bound_var (Eproj x tau n y' e) y
+| Bound_Ecase :
+    forall x y c e B,
+      bound_var e y ->
+      List.In (c, e) B ->
+      bound_var (Ecase x B) y
 | Bound_Efun1 :
     forall y defs e,
-      bound_var_fundefs y defs ->
-      bound_var y (Efun defs e)
+      bound_var_fundefs defs y ->
+      bound_var (Efun defs e) y
 | Bound_Efun2 :
     forall y defs e,
-      bound_var y e ->
-      bound_var y (Efun defs e)
+      bound_var e y ->
+      bound_var (Efun defs e) y
 | Bound_Eprim1 :
     forall x tau p ys e,
-      bound_var x (Eprim x tau p ys e)
+      bound_var (Eprim x tau p ys e) x
 | Bound_Eprim2 :
     forall y x tau p ys e,
-      bound_var y e ->
-      bound_var y (Eprim x tau p ys e)
-with bound_var_fundefs : var -> fundefs -> Prop :=
+      bound_var e y ->
+      bound_var (Eprim x tau p ys e) y
+with bound_var_fundefs : fundefs -> Ensemble var :=
 | Bound_Fcons1 :
-    forall x f tau ys e defs,  
-      x = f \/ List.In x ys ->
-      bound_var_fundefs x (Fcons f tau ys e defs)
+    forall x f tau ys e defs,
+      Ensembles.In var (Union var (Singleton var f) (FromList ys)) x ->
+      bound_var_fundefs (Fcons f tau ys e defs) x
 | Bound_Fcons2 :
     forall x f tau ys e defs,
-      bound_var_fundefs x defs ->
-      bound_var_fundefs x (Fcons f tau ys e defs)
+      bound_var_fundefs defs x ->
+      bound_var_fundefs (Fcons f tau ys e defs) x
 | Bound_Fcons3 :
     forall x f tau ys e defs,
-      bound_var x e ->
-      bound_var_fundefs x (Fcons f tau ys e defs).
+      bound_var e x ->
+      bound_var_fundefs (Fcons f tau ys e defs) x.
 
 (** unique bindings - alternative definition without lists *)
 Inductive unique_bindings : exp -> Prop :=
 | UBound_Econstr :
     forall x tau t ys e,
-      (forall x', bound_var x' e -> x <> x') ->
+      ~ (bound_var e) x ->
       unique_bindings e ->
       unique_bindings (Econstr x tau t ys e)
 | UBound_Eproj :
     forall x tau n y e,
-      (forall x', bound_var x' e -> x <> x') ->
+      ~ (bound_var e) x ->
       unique_bindings e ->
       unique_bindings (Eproj x tau n y e)
 | UBound_Efun :
     forall defs e,
       unique_bindings e ->
       unique_bindings_fundefs defs ->
-      (forall x', bound_var x' e -> ~ bound_var_fundefs x' defs) ->
+      Disjoint var (bound_var e) (bound_var_fundefs defs) ->
       unique_bindings (Efun defs e)
 | UBound_Eprim :
     forall x tau p ys e,
-      (forall x', bound_var x' e -> x <> x') ->
+      ~ (bound_var e) x ->
       unique_bindings e ->
       unique_bindings (Eprim x tau p ys e)
 with unique_bindings_fundefs : fundefs -> Prop :=
 | UBound_Fcons :
     forall f tau ys e defs,
-      (forall x', bound_var x' e -> f <> x' /\ ~ List.In x' ys) ->
+      ~ (bound_var e) f ->
+      ~ (bound_var_fundefs defs) f ->
+      Disjoint var (bound_var e) (FromList ys) ->
+      Disjoint var (bound_var_fundefs defs) (FromList ys) ->
+      Disjoint var (bound_var e) (bound_var_fundefs defs) ->
+      ~ FromList ys f ->
       unique_bindings e ->
       unique_bindings_fundefs defs ->
       unique_bindings_fundefs (Fcons f tau ys e defs)
 | UBound_Fnil :
     unique_bindings_fundefs Fnil.
 
+Lemma name_in_fundefs_bound_var_fundefs B :
+  Included var (name_in_fundefs B) (bound_var_fundefs B).
+Proof.
+  induction B; simpl.
+  - intros x H. inv H.
+    constructor. eauto. constructor 2. apply IHB; eauto.
+  - apply Included_Empty_set.
+Qed.
+
+Lemma name_in_fundefs_bound_var_Efun B2 e :
+  Included var (name_in_fundefs B2) (bound_var (Efun B2 e)).
+Proof.
+  intros x H. constructor. eapply name_in_fundefs_bound_var_fundefs. eauto.
+Qed.
+
+
+Lemma split_fds_cons_l_append_fundefs f tau xs e B1 B2 B3 : 
+  split_fds (Fcons f tau xs e B1) B2 B3 ->
+  exists B1' B2',
+    B3 = fundefs_append B1' (Fcons f tau xs e B2') /\
+    split_fds B1 B2 (fundefs_append B1' B2').
+Proof.
+  revert B1 B2. induction B3; intros B1 B2 Hspl.
+  - inv Hspl.
+    + exists Fnil, B3; eauto.
+    + edestruct IHB3 as [B1' [B2' [Heq Hspl]]]; eauto.
+      exists (Fcons v t0 l e0 B1'), B2'. rewrite Heq; split; eauto.
+      simpl; constructor; eauto.
+  - inv Hspl.
+Qed.
+
+Lemma split_fds_cons_r_append_fundefs f tau xs e B1 B2 B3 : 
+  split_fds B1 (Fcons f tau xs e B2) B3 ->
+  exists B1' B2',
+    B3 = fundefs_append B1' (Fcons f tau xs e B2') /\
+    split_fds B1 B2 (fundefs_append B1' B2').
+Proof.
+  revert B1 B2. induction B3; intros B1 B2 Hspl.
+  - inv Hspl.
+    + edestruct IHB3 as [B1' [B2' [Heq Hspl]]]; eauto.
+      exists (Fcons v t0 l e0 B1'), B2'. rewrite Heq; eauto. split; eauto.
+      simpl. constructor; eauto.
+    + exists Fnil, B3; eauto.
+  - inv Hspl.
+Qed.
+
+Lemma occurs_free_fundefs_Fcons f t xs e B :
+  Same_set var (occurs_free_fundefs (Fcons f t xs e B))
+           (Union var (Setminus var (occurs_free e)
+                                (Union var (Singleton var f)
+                                       (Union var (FromList xs) (name_in_fundefs B))))
+                  (Setminus var (occurs_free_fundefs B) (Singleton var f))).
+Proof.
+  split; intros x H; inv H; eauto.
+  - left. constructor; eauto. intros Hin. inv Hin; eauto.
+    inv H. congruence. inv H; eauto.
+  - right. constructor; eauto. intros H. inv H. congruence.
+  - inv H0. constructor; eauto. 
+    intros Hc. subst. eauto.
+  - inv H0. constructor 2; eauto. intros Hc; subst; eauto.
+Qed.
+
+Lemma split_fds_fun_in_fundefs B1 B2 B3 :
+  split_fds B1 B2 B3 ->
+  Same_set _ (fun_in_fundefs B3) (Union _ (fun_in_fundefs B1) (fun_in_fundefs B2)).
+Proof.
+  intros Hspl1. induction Hspl1; simpl.
+  - rewrite IHHspl1. rewrite Union_assoc. apply Same_set_refl.
+  - rewrite IHHspl1. rewrite (Union_sym (fun_in_fundefs lfds) (Union _ _ _)).
+    rewrite (Union_sym (fun_in_fundefs lfds)). rewrite Union_assoc.
+    apply Same_set_refl.
+  - rewrite Union_Empty_set_l. apply Same_set_refl.
+Qed.
+
+
+Lemma occurs_free_fundefs_Fnil :
+  Same_set var (occurs_free_fundefs Fnil) (Empty_set var).
+Proof.
+  split; intros x H; inv H.
+Qed.
+
+Lemma occurs_free_fundefs_big_cup B :
+  Same_set _ (occurs_free_fundefs B)
+           (big_cup (fun_in_fundefs B)
+                    (fun p =>
+                       let '(f, _, xs, e) := p in
+                       (Setminus _ (occurs_free e)
+                                 (Union _ (FromList xs) (name_in_fundefs B))))).
+Proof.
+  induction B; simpl.
+  - rewrite occurs_free_fundefs_Fcons. rewrite IHB.
+    rewrite Union_big_cup, big_cup_Singleton.
+    apply Same_set_Union_compat.
+    rewrite (Union_assoc (FromList l)), (Union_sym _ (Singleton var v)),
+            <- Union_assoc. apply Same_set_refl.
+    rewrite <- Setminus_big_cup.
+    apply Same_Set_big_cup_r. intros [[[f tau] xs] e'].
+    rewrite Setminus_Union, <- Union_assoc, (Union_sym (Singleton var v)).
+    apply Same_set_refl.
+  - rewrite occurs_free_fundefs_Fnil, big_cup_Empty_set. apply Same_set_refl.
+Qed.
+
+Lemma name_in_fundefs_big_cup_fun_in_fundefs B :
+  Same_set var (name_in_fundefs B) (big_cup (fun_in_fundefs B)
+                                            (fun p =>
+                                               let '(x, _, _, _) := p in
+                                               Singleton var x)).
+Proof.
+  induction B; simpl in *.
+  - rewrite Union_big_cup, big_cup_Singleton, IHB.
+    apply Same_set_Union_compat; eauto using Same_set_refl.
+  - rewrite big_cup_Empty_set. apply Same_set_refl.
+Qed.
+  
+Lemma Same_set_fun_in_fundefs_Same_set_occurs_free_fundefs B1 B2 :
+  Same_set _ (fun_in_fundefs B1) (fun_in_fundefs B2) ->
+  Same_set _ (occurs_free_fundefs B1) (occurs_free_fundefs B2).
+Proof.
+  rewrite !occurs_free_fundefs_big_cup. intros H.
+  apply Same_Set_big_cup; eauto.
+  intros [[[f tau] xs] e']. apply Same_set_Setminus_compat.
+  apply Same_set_refl. apply Same_set_Union_compat.
+  apply Same_set_refl. rewrite !name_in_fundefs_big_cup_fun_in_fundefs.
+  apply Same_Set_big_cup_l; eauto.
+Qed.
+  
+Lemma same_split_fds_closed_occurs_free_fundefs B1 B2 B3 B3' :
+  split_fds B1 B2 B3 ->
+  split_fds B1 B2 B3' ->
+  Same_set _ (occurs_free_fundefs B3) (occurs_free_fundefs B3').
+Proof.
+  intros Hspl1 Hspl2. rewrite !occurs_free_fundefs_big_cup.
+  apply Same_Set_big_cup.
+  - intros [[[f tau] xs] e']. apply Same_set_Setminus_compat.
+    apply Same_set_refl. apply Same_set_Union_compat.
+    apply Same_set_refl. rewrite !name_in_fundefs_big_cup_fun_in_fundefs.
+    apply Same_Set_big_cup_l; eauto. rewrite split_fds_fun_in_fundefs; eauto.
+    rewrite (split_fds_fun_in_fundefs B1 B2 B3'); eauto. apply Same_set_refl.
+  - rewrite split_fds_fun_in_fundefs; eauto.
+    rewrite (split_fds_fun_in_fundefs B1 B2 B3'); eauto. apply Same_set_refl.
+Qed.
+
+Lemma same_split_fds_closed_fundefs B1 B2 B3 B3' :
+  split_fds B1 B2 B3 ->
+  split_fds B1 B2 B3' ->
+  closed_fundefs B3 -> closed_fundefs B3'.
+Proof.
+  intros Hspl1 Hspl2 Hcl. unfold closed_fundefs in *.
+  rewrite same_split_fds_closed_occurs_free_fundefs; eauto.
+Qed.
+  
 (** The set of names of the functions in the same fix definition *)
 Fixpoint fundefs_names (defs : fundefs) : FVSet :=
   match defs with
@@ -278,7 +561,6 @@ Fixpoint fundefs_names (defs : fundefs) : FVSet :=
     | Fnil => empty
   end.
 
-  
 (** The set of free variables of an exp *)
 Fixpoint exp_fv (e : exp) : FVSet :=
   match e with
@@ -308,16 +590,596 @@ with fundefs_fv (defs : fundefs) (names : FVSet) : FVSet :=
          | Fnil => empty
        end.
 
+Lemma bound_var_fundefs_Fcons f tau xs e B1 :
+  Same_set var (bound_var_fundefs (Fcons f tau xs e B1))
+           (Union var (Singleton var f)
+                  (Union var (FromList xs)
+                         (Union var (bound_var e) (bound_var_fundefs B1)))).
+Proof.
+  split; intros x H; inv H; eauto.
+  inv H6; eauto.
+  constructor; eauto.
+  inv H0. constructor; eauto.
+  inv H. constructor 3; eauto. constructor 2; eauto.
+Qed.
+
+Lemma bound_var_fundefs_Fnil  :
+  Same_set var (bound_var_fundefs Fnil) (Empty_set var).
+Proof.
+  split; intros x H; inv H; eauto.
+Qed.
+
+
+
+Lemma split_fds_bound_vars B1 B2 B3 :
+  split_fds B1 B2 B3 ->
+  Same_set var (bound_var_fundefs B3)
+           (Union var (bound_var_fundefs B1) (bound_var_fundefs B2)).
+Proof.
+  intros Hspl. induction Hspl; simpl.
+  - rewrite !bound_var_fundefs_Fcons; rewrite IHHspl.
+    repeat rewrite <- (Union_assoc _ _ (bound_var_fundefs rfds)). apply Same_set_refl.
+  - rewrite !bound_var_fundefs_Fcons. rewrite IHHspl.
+    rewrite (Union_sym _ (Union var (Singleton var v) _)).
+    repeat rewrite <- Union_assoc. rewrite (Union_sym (bound_var_fundefs lfds)).
+    apply Same_set_refl.
+  - split; intros x H; inv H; inv H0.
+Qed.
+
+Lemma split_fds_name_in_fundefs B1 B2 B3 :
+  split_fds B1 B2 B3 ->
+  Same_set var (name_in_fundefs B3)
+           (Union var (name_in_fundefs B1) (name_in_fundefs B2)).
+Proof.
+  intros Hspl. induction Hspl; simpl.
+  - rewrite IHHspl. repeat rewrite <- Union_assoc. apply Same_set_refl.
+  - rewrite IHHspl. simpl. 
+    rewrite (Union_sym _ (Union var (Singleton var v) _)).
+    repeat rewrite <- Union_assoc. rewrite (Union_sym (name_in_fundefs lfds)).
+    apply Same_set_refl.
+  - split; intros x H; inv H; inv H0.
+Qed.
+
+Lemma split_fds_unique_bindings_fundefs_l B1 B2 B3 :
+  unique_bindings_fundefs B3 ->
+  split_fds B1 B2 B3 ->
+  unique_bindings_fundefs B1 /\ unique_bindings_fundefs B2 /\
+  Disjoint var (bound_var_fundefs B1) (bound_var_fundefs B2).
+Proof.
+  intros Hun Hspl. induction Hspl; simpl.
+  - inv Hun. edestruct IHHspl as [H1 [H2 H3]]; eauto.
+    erewrite (split_fds_bound_vars _ _ lrfds) in H8, H7; eauto.
+    repeat split; eauto. constructor; eauto.
+    intros Hc. apply H5. eapply split_fds_bound_vars; eauto.
+    apply Disjoint_sym in H8. eapply Disjoint_Union_l; eauto.
+    apply Disjoint_sym in H8. eapply Disjoint_sym.
+    eapply Disjoint_Union_l; eauto.
+    intros x Hin. inv Hin. rewrite bound_var_fundefs_Fcons in H.
+    inv H. inv H12. eapply H5. eapply split_fds_bound_vars; eauto.
+    inv H12. eapply H7. constructor; eauto.
+    inv H. eapply H8; constructor; eauto.
+    eapply H3; constructor; eauto.
+  - inv Hun. edestruct IHHspl as [H1 [H2 H3]]; eauto.
+    erewrite (split_fds_bound_vars _ _ lrfds) in H8, H7; eauto.
+    repeat split; eauto. constructor; eauto.
+    intros Hc. apply H5. eapply split_fds_bound_vars; eauto.
+    apply Disjoint_sym in H8. eapply Disjoint_Union_r; eauto.
+    apply Disjoint_sym in H8. eapply Disjoint_sym.
+    eapply Disjoint_Union_r; eauto.
+    intros x Hin. inv Hin. rewrite bound_var_fundefs_Fcons in H0.
+    inv H0. inv H12. eapply H5. eapply split_fds_bound_vars; eauto.
+    inv H12. eapply H7. constructor; eauto.
+    inv H0. eapply H8; constructor; eauto.
+    eapply H3; constructor; eauto.
+  - split; try constructor; eauto. rewrite bound_var_fundefs_Fnil at 1.
+    apply Disjoint_Empty_set_l.
+Qed.
+
+Lemma split_fds_unique_bindings_fundefs_r B1 B2 B3 :
+  unique_bindings_fundefs B1 -> unique_bindings_fundefs B2 ->
+  Disjoint var (bound_var_fundefs B1) (bound_var_fundefs B2) ->
+  split_fds B1 B2 B3 ->
+  unique_bindings_fundefs B3.
+Proof.
+  intros Hun1 Hun2 HD Hspl. induction Hspl; simpl.
+  - inv Hun1. constructor; eauto.
+    + intros Hc. apply H5. 
+      eapply (split_fds_bound_vars) in Hc; eauto. inv Hc; eauto.
+      inv HD. exfalso. eapply H0. constructor; eauto.
+      constructor; eauto.
+    + rewrite split_fds_bound_vars; eauto.
+      constructor. intros x H. inv H. inv H0; eauto.
+      eapply H7. constructor; eauto.
+      eapply HD; constructor; eauto. constructor; eauto.
+    + rewrite split_fds_bound_vars; eauto.
+      constructor. intros x H. inv H. inv H1; eauto.
+      eapply H8. constructor; eauto. 
+      eapply HD; constructor; eauto. constructor 3; eauto.
+    + eapply IHHspl; eauto. rewrite bound_var_fundefs_Fcons in HD.
+      repeat apply Disjoint_Union_r in HD; eauto.
+  - inv Hun2. constructor; eauto.
+    + intros Hc. apply H5. 
+      eapply (split_fds_bound_vars) in Hc; eauto. inv Hc; eauto.
+      inv HD. exfalso. eapply H0. constructor; eauto.
+      constructor; eauto.
+    + rewrite split_fds_bound_vars; eauto.
+      constructor. intros x H. inv H. inv H0; eauto.
+      eapply HD; constructor; eauto. constructor; eauto.
+      eapply H7. constructor; eauto.
+    + rewrite split_fds_bound_vars; eauto.
+      constructor. intros x H. inv H. inv H1; eauto.
+      eapply HD; constructor; eauto. constructor 3; eauto.
+      eapply H8. constructor; eauto. 
+    + eapply IHHspl; eauto. rewrite bound_var_fundefs_Fcons in HD.
+      apply Disjoint_sym in HD. repeat apply Disjoint_Union_r in HD; eauto.
+      apply Disjoint_sym; eauto.
+  - constructor.
+Qed.
+
+Lemma find_def_not_name_in_fundefs f B1 :
+  ~ name_in_fundefs B1 f ->
+  find_def f B1 = None.
+Proof.
+  induction B1; eauto; intros H.
+  simpl. destruct (M.elt_eq f v); subst.
+  exfalso. apply H; left; eauto.
+  apply IHB1. intros H'. apply H. constructor 2; eauto.
+Qed.
+      
+
+Lemma fun_in_fundefs_name_in_fundefs f tau xs e B :
+    fun_in_fundefs B (f, tau, xs, e) ->
+    name_in_fundefs B f.
+Proof.
+  induction B; intros H; eauto; try now inv H.
+  inv H. inv H0. constructor; eauto.
+  constructor 2; eauto.
+Qed.
+
+Lemma fundefs_append_unique_bindings_l B1 B2 B3 :
+  unique_bindings_fundefs B3 ->
+  fundefs_append B1 B2 = B3 ->
+  unique_bindings_fundefs B1 /\
+  unique_bindings_fundefs B2 /\
+  Disjoint var (bound_var_fundefs B1) (bound_var_fundefs B2).
+Proof.
+  intros. edestruct split_fds_unique_bindings_fundefs_l; eauto.
+  apply fundefs_append_split_fds; eauto.
+Qed.
+
+Lemma fundefs_append_unique_bindings_r B1 B2 B3 :
+  fundefs_append B1 B2 = B3 ->
+  unique_bindings_fundefs B1 ->
+  unique_bindings_fundefs B2 ->
+  Disjoint var (bound_var_fundefs B1) (bound_var_fundefs B2) ->
+  unique_bindings_fundefs B3.
+Proof.
+  intros.
+  eapply split_fds_unique_bindings_fundefs_r;
+    [ apply H0 | | | ]; eauto.
+  apply fundefs_append_split_fds; eauto.
+Qed.
+
+
+Lemma fundefs_append_bound_vars B1 B2 B3 :
+  fundefs_append B1 B2 = B3 ->
+  Same_set var (bound_var_fundefs B3)
+           (Union var (bound_var_fundefs B1) (bound_var_fundefs B2)).
+Proof.
+  intros H. eapply split_fds_bound_vars. eapply fundefs_append_split_fds; eauto.
+Qed.
+
+Lemma fundefs_append_fun_in_fundefs B1 B2 B3 :
+  fundefs_append B1 B2 = B3 ->
+  Same_set _ (fun_in_fundefs B3)
+           (Union _ (fun_in_fundefs B1) (fun_in_fundefs B2)).
+Proof.
+  intros H. eapply split_fds_fun_in_fundefs.
+  eapply fundefs_append_split_fds; eauto.
+Qed.
+
+Lemma fun_in_fundefs_Fcons_Disjoint f tau xs e B :
+  unique_bindings_fundefs (Fcons f tau xs e B) ->
+  ~ (name_in_fundefs B f).
+Proof.
+  intros Hun Hc. inv Hun.
+  apply H5. now eapply name_in_fundefs_bound_var_fundefs.
+Qed.
+
+                    
+Lemma fun_in_fundefs_unique_bindings_split f tau xs e B :
+  fun_in_fundefs B (f, tau, xs, e) ->
+  unique_bindings_fundefs B ->
+  exists B1 B2,
+    B = fundefs_append B1 (Fcons f tau xs e B2) /\
+    ~ name_in_fundefs B1 f /\
+    Same_set _ (Union _ (fun_in_fundefs B1) (fun_in_fundefs B2))
+             (Setminus _ (fun_in_fundefs B) (Singleton _ (f, tau, xs, e))) /\
+    unique_bindings_fundefs (fundefs_append B1 B2).
+Proof.
+  intros H Hun. induction B.
+  - simpl in H.
+    destruct (var_dec v f); subst.
+    + inv H. inv H0.
+      * exists Fnil. eexists. split; simpl; eauto.
+        split; try (now intros Hc; inv Hc). split; try (now inv Hun; eauto).
+        rewrite Union_Empty_set_r, Setminus_Union_distr, Setminus_Empty_set,
+        Union_Empty_set_r. apply Same_set_sym. eapply Setminus_Disjoint.
+        apply Disjoint_Singleton. intros Hc.
+        apply fun_in_fundefs_name_in_fundefs in Hc.
+        eapply fun_in_fundefs_Fcons_Disjoint; eauto.
+      * exfalso. inv Hun. apply H6. eapply name_in_fundefs_bound_var_fundefs.
+        eapply fun_in_fundefs_name_in_fundefs; eauto.
+    + inv H. inv H0. congruence. inv Hun; eauto.
+      edestruct IHB as [B1 [B2 [Heq [Hn [Hs Hun']]]]]; eauto.
+      edestruct fundefs_append_unique_bindings_l as [H1 [H2 H3]];
+        [ apply H12 | | ]; eauto.
+      exists (Fcons v t0 l e0 B1), B2. rewrite Heq. split; eauto.
+      split; [| split ].
+      * intros H. apply Hn. inv H; eauto. inv H4. congruence.
+      * simpl. rewrite Setminus_Union_distr, <- Union_assoc.
+        apply Same_set_Union_compat.
+        apply Same_set_sym. eapply Setminus_Disjoint.
+        apply Disjoint_Singleton. intros Hc. inv Hc. congruence.
+        apply Same_set_sym. 
+        rewrite fundefs_append_fun_in_fundefs; eauto. simpl.
+        rewrite !Setminus_Union_distr, Setminus_Empty_set, Union_Empty_set_r,
+        <- Setminus_Union_distr.
+        eapply Setminus_Disjoint. apply Disjoint_Union.
+        eapply Disjoint_Singleton. intros Hc. eapply H3.
+        constructor. eapply name_in_fundefs_bound_var_fundefs.
+        eapply fun_in_fundefs_name_in_fundefs; eauto.
+        rewrite bound_var_fundefs_Fcons; left. eauto.
+        eapply Disjoint_Singleton. intros Hc. inv H2. eapply H17.
+        eapply name_in_fundefs_bound_var_fundefs.
+        eapply fun_in_fundefs_name_in_fundefs; eauto.
+      * simpl. constructor; eauto.
+        intros H. apply H6. eapply fundefs_append_bound_vars; eauto.
+        eapply fundefs_append_bound_vars in H; [| eauto ].
+        rewrite bound_var_fundefs_Fcons. inv H; eauto.
+        constructor. intros x Hc. eapply H8. inv Hc.
+        constructor; eauto.
+        rewrite fundefs_append_bound_vars in H; [| eauto ].
+        eapply fundefs_append_bound_vars; eauto.
+        rewrite bound_var_fundefs_Fcons. inv H; eauto.
+        eapply Disjoint_Included_r; eauto.
+        rewrite Heq, fundefs_append_bound_vars; eauto.
+        rewrite (fundefs_append_bound_vars B1 (Fcons f tau xs e B2)
+                                           (fundefs_append B1 (Fcons f tau xs e B2))); eauto.
+        apply Included_Union_compat; eauto using Included_refl.
+        rewrite bound_var_fundefs_Fcons.
+        rewrite !Union_assoc, Union_sym. apply Included_Union_l.
+  - inv H.
+Qed.
+
+Lemma fundefs_append_name_in_fundefs B1 B2 B3 :
+  fundefs_append B1 B2 = B3 ->
+  Same_set var (name_in_fundefs B3)
+           (Union var (name_in_fundefs B1) (name_in_fundefs B2)).
+Proof.
+  revert B3. induction B1; intros B3 Heq; simpl.
+  - destruct B3. simpl in Heq. inv Heq. simpl. 
+    rewrite IHB1; eauto. rewrite Union_assoc. apply Same_set_refl.
+    inv Heq.
+  - inv Heq. simpl. rewrite Union_Empty_set_r.
+    apply Same_set_refl.
+Qed.
+
+Lemma find_def_Included_fun_in_fundefs f B B' :
+  unique_bindings_fundefs B ->
+  unique_bindings_fundefs B' ->
+  Included _ (fun_in_fundefs B) (fun_in_fundefs B') ->
+  name_in_fundefs B f ->
+  find_def f B = find_def f B'.
+Proof.
+  revert B'. induction B; simpl; intros B' Hun Hun' H Hn.
+  - edestruct fun_in_fundefs_unique_bindings_split
+      as [B1 [B1' [Heq [Hn' [HS' Hun1]]]]]; eauto.
+    eapply H. left. eauto.
+    rewrite Heq. destruct (M.elt_eq f v); subst.
+    + erewrite find_def_fundefs_append_r.
+      simpl; destruct (M.elt_eq v v); try congruence.
+      simpl; destruct (M.elt_eq v v); try congruence. eauto.
+      apply find_def_not_name_in_fundefs.
+      intros Hc. apply Hn'; eauto.
+    + rewrite find_def_fundefs_append_Fcons_neq; eauto. eapply IHB; eauto.
+      inv Hun; eauto.
+      rewrite (fundefs_append_fun_in_fundefs B1 B1' (fundefs_append B1 B1')); eauto.
+      eapply Included_trans; [| inv HS'; eauto].
+      rewrite <- (Setminus_Disjoint (fun_in_fundefs B) (Singleton _ (v, t0, l, e))).
+      rewrite <- Setminus_Union_Inlcluded; eauto using Included_refl.
+      eapply Included_Setminus_compat; eauto using Included_refl.
+      now rewrite Union_sym.  
+      eapply Disjoint_Singleton. inv Hun; eauto. intros Hc. apply H6.
+      apply name_in_fundefs_bound_var_fundefs.
+      now eapply fun_in_fundefs_name_in_fundefs; eauto.
+      inv Hn. inv H0; try congruence. eauto.
+  - destruct B'; eauto. inv Hn.
+Qed.
+
+
+Lemma find_def_Same_set_fun_in_fundefs f B B' :
+  unique_bindings_fundefs B ->
+  unique_bindings_fundefs B' ->
+  Same_set _ (fun_in_fundefs B) (fun_in_fundefs B') ->
+  find_def f B = find_def f B'.
+Proof.
+  intros Hun1 Hun2 HS.
+  destruct (@Dec _ _ (Decidable_name_in_fundefs B) f).
+  - inv HS. eapply find_def_Included_fun_in_fundefs; eauto.
+  - rewrite !name_in_fundefs_find_def_None; eauto.
+    intros Hn. apply H.
+    apply name_in_fundefs_big_cup_fun_in_fundefs in Hn.
+    destruct Hn as [[[[f' t] xs] e] [H1 H2]]. inv H2.
+    eapply fun_in_fundefs_name_in_fundefs. now eapply HS; eauto.
+Qed.
+
+Lemma split_fds_occurs_free_fundefs B1 B2 B3 :
+  split_fds B1 B2 B3 ->
+  Same_set var (occurs_free_fundefs B3)
+           (Union _ (Setminus _ (occurs_free_fundefs B1) (name_in_fundefs B2))
+                  (Setminus _ (occurs_free_fundefs B2) (name_in_fundefs B1))).
+Proof.
+  intros H1.
+  rewrite !occurs_free_fundefs_big_cup.
+  rewrite <- !Setminus_big_cup.
+  eapply Same_set_trans with
+  (s2 := Union var
+               (big_cup (fun_in_fundefs B1) _)
+               (big_cup (fun_in_fundefs B2) _)).
+  rewrite <- Union_big_cup.
+  eapply Same_Set_big_cup_l. rewrite split_fds_fun_in_fundefs; eauto.
+  apply Same_set_refl.
+  eapply Same_set_Union_compat; eapply Same_Set_big_cup_r;
+  intros [[[f tau] xs] e]; rewrite Setminus_Union; rewrite <- Union_assoc.
+  rewrite split_fds_name_in_fundefs; eauto. apply Same_set_refl.
+  rewrite (Union_sym (name_in_fundefs B2) (name_in_fundefs B1)).
+  rewrite split_fds_name_in_fundefs; eauto. apply Same_set_refl.
+Qed.
+
+Lemma split_fds_closed_fundefs B1 B2 B3 :
+  split_fds B1 B2 B3 ->
+  closed_fundefs B1 ->
+  closed_fundefs B2 ->
+  closed_fundefs B3.
+Proof.
+  intros H1 H2 H3. unfold closed_fundefs in *.
+  rewrite split_fds_occurs_free_fundefs; eauto.
+  rewrite H2, H3. rewrite !Setminus_Included_Empty_set.
+  rewrite Union_Empty_set_r. apply Same_set_refl.
+  intros x Hc; inv Hc. intros x Hc; inv Hc.
+Qed.
+
+Lemma bound_var_Efun B e :
+  Same_set var (bound_var (Efun B e))
+           (Union var (bound_var_fundefs B) (bound_var e)).
+Proof.
+  split; intros x H; inv H; eauto.
+  apply Bound_Efun1; eauto. apply Bound_Efun2; eauto.
+Qed.
+  
+Lemma unique_bindings_hoist B1 B2 B3 f tau xs e B B' :
+  split_fds B1 (Fcons f tau xs (Efun B3 e) Fnil) B ->
+  split_fds B1 (Fcons f tau xs e Fnil) B2 ->
+  split_fds B3 B2 B' ->
+  unique_bindings_fundefs B ->
+  unique_bindings_fundefs B'.
+Proof.
+  intros Hsp1 Hsp2 Hsp3 Hun.
+  edestruct split_fds_unique_bindings_fundefs_l as [H1 [H2 H3]]; eauto.
+  assert (Hun2 : unique_bindings_fundefs B2).
+  { eapply split_fds_unique_bindings_fundefs_r; [ | | | apply Hsp2 ]; eauto.
+    inv H2. rewrite bound_var_Efun in *. constructor; eauto. intros H. apply H7.
+    apply Bound_Efun2; eauto.
+    eapply Disjoint_Union_r; eauto.
+    eapply Disjoint_Union_r; eauto.
+    inv H13; eauto.
+    rewrite bound_var_fundefs_Fcons in *.
+    eapply Disjoint_Included_r; eauto.
+    repeat apply Included_Union_compat; eauto using Included_refl.
+    rewrite bound_var_Efun. apply Included_Union_r. }
+  edestruct split_fds_unique_bindings_fundefs_l as [H1' [H2' H3']]; eauto.
+  eapply split_fds_unique_bindings_fundefs_r; [ | | | eauto]; eauto.
+  inv H2. inv H13; eauto.
+  inv H2.
+  rewrite (split_fds_bound_vars B1 (Fcons f tau xs e Fnil) B2); eauto.
+  rewrite bound_var_fundefs_Fcons in *. rewrite bound_var_Efun in *.
+  apply Disjoint_sym. apply Disjoint_Union.
+  eapply Disjoint_Included_r; [| eapply H3 ].
+  rewrite Union_assoc, Union_sym, <- !Union_assoc.
+  apply Included_Union_l.
+  apply Disjoint_Union. eapply Disjoint_sym. eapply Disjoint_Singleton.
+  intros Hc. apply H7. eapply Bound_Efun1; eauto.
+  apply Disjoint_Union. eapply Disjoint_sym.
+  eapply Disjoint_Included_l; [| eapply H9 ].
+  apply Included_Union_l.
+  rewrite bound_var_fundefs_Fnil, Union_Empty_set_l.
+  now inv H13.
+Qed.
+
+Lemma unique_bindings_split_fds_Fcons_fundefs_append B1 B2 B3 B f tau xs e  :
+  split_fds B1 (Fcons f tau xs e Fnil) B3 ->
+  split_fds B2 B3 B ->
+  unique_bindings_fundefs B ->
+  unique_bindings_fundefs (fundefs_append (Fcons f tau xs e B1) B2).
+Proof.
+  intros H1 H2 Hun.
+  edestruct split_fds_unique_bindings_fundefs_l as [H1' [H2' H3']];
+  [| apply H2 |]; eauto.
+  edestruct split_fds_unique_bindings_fundefs_l as [H4' [H5' H6']];
+    [| apply H1 |]; eauto.
+  eapply fundefs_append_unique_bindings_r; eauto.
+  eapply fundefs_append_unique_bindings_r
+  with (B1 := Fcons f tau xs e Fnil) (B2 := B1); eauto.
+  inv H5'; eauto. now apply Disjoint_sym.
+  rewrite bound_var_fundefs_Fcons.
+  rewrite (split_fds_bound_vars B1 (Fcons f tau xs e Fnil) B3) in H3'; eauto.
+  rewrite bound_var_fundefs_Fcons, bound_var_fundefs_Fnil,
+  Union_Empty_set_l in H3'.
+  rewrite !Union_assoc, Union_sym, <- !Union_assoc. now apply Disjoint_sym.
+Qed.
+
+Lemma split_fds_funs_in_fundef_l B1 B2 B3 B :
+  split_fds B1 B2 B3 ->
+  funs_in_fundef B B1 ->
+  funs_in_fundef B B3.
+Proof.
+  intros Hsp Hf. induction Hsp.
+  - inv Hf. constructor; eauto.
+    constructor 2; eauto.
+  - constructor 2; eauto.
+  - inv Hf.
+Qed.
+
+Lemma split_fds_funs_in_fundef_r B1 B2 B3 B :
+  split_fds B1 B2 B3 ->
+  funs_in_fundef B B2 ->
+  funs_in_fundef B B3.
+Proof.
+  intros Hsp Hf. induction Hsp.
+  - constructor 2; eauto.
+  - inv Hf. constructor; eauto.
+    constructor 2; eauto.
+  - inv Hf.
+Qed.
+
+Lemma unique_bindings_split_fds_fundfes_append B1 B2 B3 :
+  split_fds B1 B2 B3 ->
+  unique_bindings_fundefs B3 ->
+  unique_bindings_fundefs (fundefs_append B1 B2).
+Proof.
+  intros Hspl Hun.
+  edestruct split_fds_unique_bindings_fundefs_l as [H1 [H2 H3]]; eauto.
+  eapply fundefs_append_unique_bindings_r; eauto.
+Qed.
+
+Lemma split_fds_fundefs_append_fun_in_fundefs B1 B2 B3 B4 B : 
+  split_fds B1 B2 B4 ->
+  split_fds B3 B4 B ->
+  Same_set _ (fun_in_fundefs (fundefs_append (fundefs_append B2 B1) B3))
+           (fun_in_fundefs B).
+Proof.
+  intros H1 H2.
+  rewrite (split_fds_fun_in_fundefs B3 B4 B); eauto;
+  rewrite (split_fds_fun_in_fundefs B1 B2 B4); eauto.
+  rewrite (fundefs_append_fun_in_fundefs (fundefs_append B2 B1) B3); eauto.
+  rewrite (fundefs_append_fun_in_fundefs B2 B1); eauto.
+  rewrite (Union_sym (Union _ _ _) _),
+  (Union_sym (fun_in_fundefs B2) (fun_in_fundefs B1)).
+  apply Same_set_refl.
+Qed.
+
+Lemma find_def_split_fds f B1 B2 B3 B3' :
+  split_fds B1 B2 B3 ->
+  split_fds B1 B2 B3' ->
+  unique_bindings_fundefs B3 ->
+  find_def f B3 = find_def f B3'.
+Proof.
+  intros Hspl1 Hspl2 Hun.
+  edestruct split_fds_unique_bindings_fundefs_l as [H1 [H2 H3]]; eauto.
+  specialize (split_fds_unique_bindings_fundefs_r _ _ _ H1 H2 H3 Hspl2).
+  clear H1 H2 H3.
+  revert B3' Hspl2. induction Hspl1; intros B3' Hspl2 Hun'.
+  - simpl. destruct (M.elt_eq f v); subst.
+    + edestruct split_fds_cons_l_append_fundefs as [B1' [B2' [Heq Hspl3]]]; eauto.
+      erewrite Heq, find_def_fundefs_append_r;
+        try (now simpl; destruct (M.elt_eq v v); try congruence; eauto).
+      eapply find_def_not_name_in_fundefs. intros Hc.
+      symmetry in Heq. apply fundefs_append_split_fds in Heq.
+      edestruct split_fds_unique_bindings_fundefs_l as [H1 [H2 H3]]; eauto.
+      eapply H3. constructor; eauto. apply name_in_fundefs_bound_var_fundefs; eauto.
+      rewrite bound_var_fundefs_Fcons. left; eauto.
+    + edestruct split_fds_cons_l_append_fundefs as [B1' [B2' [Heq Hspl3]]]; eauto.
+      erewrite Heq. rewrite find_def_fundefs_append_Fcons_neq; eauto.
+      inv Hun. apply IHHspl1; eauto.
+      edestruct split_fds_unique_bindings_fundefs_l as [H1 [H2 H3]];
+        [| apply Hspl1 |]; eauto.
+      now specialize (split_fds_unique_bindings_fundefs_r _ _ _ H1 H2 H3 Hspl3).
+  - simpl. destruct (M.elt_eq f v); subst.
+    + edestruct split_fds_cons_r_append_fundefs as [B1' [B2' [Heq Hspl3]]]; eauto.
+      erewrite Heq, find_def_fundefs_append_r;
+        try (now simpl; destruct (M.elt_eq v v); try congruence; eauto).
+      eapply find_def_not_name_in_fundefs. intros Hc.
+      symmetry in Heq. apply fundefs_append_split_fds in Heq.
+      edestruct split_fds_unique_bindings_fundefs_l as [H1 [H2 H3]]; eauto.
+      eapply H3. constructor; eauto. apply name_in_fundefs_bound_var_fundefs; eauto.
+      rewrite bound_var_fundefs_Fcons. left; eauto.
+    + edestruct split_fds_cons_r_append_fundefs as [B1' [B2' [Heq Hspl3]]]; eauto.
+      erewrite Heq. rewrite find_def_fundefs_append_Fcons_neq; eauto.
+      inv Hun. apply IHHspl1; eauto.
+      edestruct split_fds_unique_bindings_fundefs_l as [H1 [H2 H3]];
+        [| apply Hspl1 |]; eauto.
+      now specialize (split_fds_unique_bindings_fundefs_r _ _ _ H1 H2 H3 Hspl3).
+  - inv Hspl2; eauto.
+Qed.
+
+Lemma def_funs_spec x v B B' rho rho' :
+  M.get x (def_funs B' B rho rho') = Some v ->
+  (name_in_fundefs B x /\ v = cps.Vfun rho B' x) \/
+  (~ name_in_fundefs B x /\ M.get x rho' = Some v).
+Proof.
+  induction B; intros Hget.
+  - simpl in Hget. rewrite M.gsspec in Hget. destruct (Coqlib.peq x v0).
+    + inv Hget. left. split; eauto. constructor; eauto.
+    + destruct (IHB Hget) as [[H1 H2] | [H1 H2]]; eauto.
+      * left. split; eauto. constructor 2; eauto.
+      * right. split; eauto. intros Hc. inv Hc; try (inv H; congruence); eauto.
+  - simpl in Hget. right. split; eauto. intros Hc; inv Hc.
+Qed.
+
+Lemma def_funs_eq x B B' rho rho' :
+  name_in_fundefs B x ->
+  M.get x (def_funs B' B rho rho') = Some (cps.Vfun rho B' x).
+Proof.
+  induction B; intros Hin; inv Hin.
+  - simpl. inv H; rewrite M.gss. eauto.
+  - simpl. rewrite M.gsspec. destruct (Coqlib.peq x v); subst; eauto.
+Qed.
+
+Lemma def_funs_neq x B B' rho rho' :
+  ~ name_in_fundefs B x ->
+  M.get x (def_funs B' B rho rho') = M.get x rho'.
+Proof.
+  induction B; intros Hin; simpl; eauto.
+  rewrite M.gsspec. destruct (Coqlib.peq x v); subst; eauto.
+  exfalso. apply Hin. constructor; eauto. eapply IHB.
+  intros Hc.  eapply Hin. constructor 2; eauto.
+Qed.
+
+Lemma get_fundefs y v B B' rho :
+  M.get y rho = Some v -> ~ name_in_fundefs B y ->
+  M.get y (def_funs B' B rho rho) = Some v.
+Proof.
+  intros Hget Hn.
+  rewrite def_funs_neq; eauto.
+Qed.
+
+Lemma getlist_fundefs ys vs B B' rho :
+  getlist ys rho = Some vs ->
+  (forall y, List.In y ys -> ~ name_in_fundefs B y) ->
+  getlist ys (def_funs B' B rho rho) = Some vs.
+Proof.
+  revert rho vs. induction ys; intros rho vs Hget Hall.
+  - now inv Hget.
+  - simpl in Hget.
+    destruct (M.get a rho) eqn:Heq1; try discriminate.
+    destruct (getlist ys rho) eqn:Heq2; try discriminate. inv Hget.
+    simpl. erewrite IHys; eauto. erewrite get_fundefs; eauto.
+    intros Hc. eapply Hall; eauto. left; eauto.
+    intros y Hin Hc. eapply Hall; eauto. right; eauto.
+Qed.
+
+
 (** Equivalence of computational and inductive FV definitions *)
 
 (** fundefs_names correct w.r.t name_in_fundefs *)
 Lemma fundefs_names_correct (defs : fundefs) :
-  forall f, In f (fundefs_names defs) <-> name_in_fundefs f defs.
+  forall f, In f (fundefs_names defs) <-> name_in_fundefs defs f.
 Proof.
   induction defs; simpl; intros f; split; intros H; try now inv H.
-  - apply add_spec in H. inv H; eauto.
+  - apply add_spec in H. inv H; eauto. left; eauto.
     right. eapply IHdefs; eauto.
-  - apply add_spec. inv H; eauto.
+  - apply add_spec. inv H; eauto. inv H0; eauto.
     right. eapply IHdefs; eauto.
 Qed.
 
@@ -344,7 +1206,6 @@ Proof.
   - inv HIn.
   - apply_set_specs_ctx; eauto.
 Qed.
-
 
 Lemma In_fold_left_l {A} (f : A -> FVSet) (l : list A)
       (si : FVSet) x:
@@ -419,10 +1280,10 @@ Qed.
 (** correctness of exp_fv and fundefs_fv w.r.t occurs_free
     and occurs_free_def *)
 Lemma exp_fv_fundefs_fv_correct :
-  (forall e x, In x (exp_fv e) <-> occurs_free x e) /\
+  (forall e x, In x (exp_fv e) <-> occurs_free e x) /\
   (forall defs x,
      In x (fundefs_fv defs (fundefs_names defs)) <->
-     occurs_free_fundefs x defs).
+     occurs_free_fundefs defs x).
 Proof.
   exp_defs_induction IHe IHl IHdefs; simpl; intros x; split; intros H.
   - repeat apply_set_specs_ctx.
@@ -439,7 +1300,7 @@ Proof.
   - inv H.
     + eapply In_fold_left. apply_set_specs. right; constructor; eauto.
     + apply In_fold_left. apply_set_specs; left. apply IHe; eauto.
-    + apply IHl in H2. simpl in H2.
+    + apply IHl in H5. simpl in H5.
       eapply In_fold_left_weaken; eauto.
       apply Subset_union_mon_r. apply Subset_refl.
   - repeat apply_set_specs_ctx.
@@ -453,7 +1314,7 @@ Proof.
       eapply IHe; eauto.
   - inv H; repeat apply_set_specs; eauto.
     + right. apply_set_specs; eauto. apply IHe; eauto.
-      intros Hc; apply H3; apply fundefs_names_correct; eauto.
+      intros Hc; apply H2; apply fundefs_names_correct; eauto.
     + left. eapply IHdefs; eauto.
   - repeat apply_set_specs_ctx; constructor; eauto.
   - inv H; apply_set_specs; eauto. left. apply_set_specs; eauto.
